Lp2lc/Active/Util.lean
@@ -73,15 +73,16 @@ reconstruction to identifiers carrying evidence for the auxiliary instance.
 -/
 class Aux {UId : TIndex} {V : Type}
     (outer : UIdEquiv UId V) (M : V → Sort u) where
-  Receipt : UId → Prop
-  getEv : (bundle : PSigma M) → Receipt (outer.getUId bundle.fst)
-  invEv : (ev: PSigma Receipt) → M (outer.inv ev.fst)
+  Ev : UId → Prop
+  Receipt := PSigma Ev -- TODO: make this a final method
+  getEv : (bundle : PSigma M) → Ev (outer.getUId bundle.fst)
+  invEv : (ev: Receipt) → M (outer.inv ev.fst)
 
 namespace Aux
 
 section variable {UId : TIndex} {V : Type} {outer : UIdEquiv UId V} {M : V → Sort u} (self : Aux outer M)
 
-abbrev AuxUId := PSigma self.Receipt
+abbrev AuxUId := PSigma self.Ev
 
 /-- Saving membership and reconstructing metadata preserves the original value. -/
 @[simp]
